TestModels/Streaming/src/SimpleStreamingImpl.dfy
@@ -5,8 +5,9 @@ include "../Model/SimpleStreamingTypes.dfy"
 include "Chunker.dfy"
 module {:options "/functionSyntax:4" } SimpleStreamingImpl refines AbstractSimpleStreamingOperations {
 
-  import Std.Enumerators
-  import Std.Aggregators
+  import Std.Actions
+  import Std.Producers
+  import Std.Consumers
   import Std.Collections.Seq
   import opened Chunker
   
@@ -22,30 +23,18 @@ module {:options "/functionSyntax:4" } SimpleStreamingImpl refines AbstractSimpl
   method CountBits ( config: InternalConfig , input: CountBitsInput )
     returns (output: Result<CountBitsOutput, Error>)
   {
-    var counter := new Aggregators.FoldingAccumulator<BoundedInts.bytes, int>(0, (sum, byte) => sum + BytesBitCount(byte));
+    var counter := new Consumers.FoldingConsumer(0, SumBits);
+    var counterTotalProof := new Consumers.FoldingConsumerTotalActionProof(counter);
  
-    Enumerators.ForEach(input.bits, counter);
+    input.bits.ForEachRemaining(counter, counterTotalProof);
 
-    // Should really have the FoldingAccumulator fail instead,
+    // Should really have the FoldingConsumer fail instead,
     // but this is a simpler correct approach.
     if 0 <= counter.value < INT32_MAX_LIMIT {
       return Success(CountBitsOutput(sum := counter.value as int32));
     } else {
       return Failure(OverflowError(message := "Ah crap"));
     }
-  }
-
-  function BytesBitCount(b: BoundedInts.bytes): int {
-    Seq.FoldLeft((sum, byte) => sum + BitCount(byte), 0 as int, b)
-  }
-
-  function BitCount(x: BoundedInts.uint8): int {
-    if x == 0 then
-      0
-    else if x % 2 == 1 then
-      1 + BitCount(x / 2)
-    else
-      BitCount(x / 2)
   }
 
   predicate BinaryOfEnsuresPublicly(input: BinaryOfInput , output: Result<BinaryOfOutput, Error>)
@@ -58,9 +47,9 @@ module {:options "/functionSyntax:4" } SimpleStreamingImpl refines AbstractSimpl
 
   {
     // TODO: Actually compute the binary
-    var fakeBinary: seq<BoundedInts.bytes> := [[12], [34, 56]];
-    var fakeBinaryEnumerator := new Enumerators.SeqEnumerator(fakeBinary);
-    var fakeBinaryStream := new EnumeratorDataStream(fakeBinaryEnumerator, 3 as BoundedInts.uint64);
+    var fakeBinary := [Success([12]), Success([34, 56])];
+    var fakeBinaryEnumerator := new Producers.SeqReader(fakeBinary);
+    var fakeBinaryStream := new ProducerDataStream(fakeBinaryEnumerator, 3 as BoundedInts.uint64);
     
     return Success(BinaryOfOutput(binary := fakeBinaryStream));
   }
@@ -74,7 +63,7 @@ module {:options "/functionSyntax:4" } SimpleStreamingImpl refines AbstractSimpl
   {
     // TODO: for now
     assume {:axiom} input.bytesIn.history == [];
-    var chunker := new Chunker(input.bytesIn, input.chunkSize);
+    var chunker := new Chunker(input.chunkSize);
     var chunkerStream := new EnumeratorDataStream(chunker, input.bytesIn.ContentLength());
     
     return Success(ChunksOutput(bytesOut := chunkerStream));
